examples/ListaPersonas.dfy
@@ -1,0 +1,39 @@
+include "../src/linear/layer2/ArrayList.dfy"
+include "iterators/FillArray.dfy"
+
+class Person{
+  var id:nat;
+  var age:nat;
+  var name:string;
+
+  constructor(i:nat,a:nat,n:string)
+  {
+    id:=i;
+    age:=a;
+    name:=n;
+  }
+  method changeName(n:string)
+  modifies this
+  {
+   name:=n;
+
+  }
+}
+
+method Test(l:List<Person>,persons:array<Person>)
+modifies l, l.Repr(),persons
+requires allocated(l.Repr())
+requires l.Valid()
+
+requires {persons} !! {l}+l.Repr()
+requires persons.Length == |l.Model()|
+
+ensures l.Valid()
+ensures persons[..] == l.Model()
+
+{
+  FillArray(l,persons);
+  var clara := new Person(1,48,"Clara");
+  l.PushBack(clara);
+  var _ := l.PopBack();
+}
