examples/iterators/FillArray.dfy
@@ -4,26 +4,29 @@ include "../../src/linear/layer2/ArrayList.dfy"
 
 method FillArray<A>(l: List<A>, v: array<A>)
   modifies l,l.Repr(), v
-  requires {v} !! {l}+l.Repr()
+  requires allocated(l.Repr())
+
   requires l.Valid()
+  requires {v} !! {l}+l.Repr()
   requires v.Length == |l.Model()|
-  requires forall x | x in l.Repr() :: allocated(x)
 
   ensures l.Valid()
   ensures l.Model() == old(l.Model())
   ensures v[..] == l.Model()
 
+
+  ensures fresh(l.Repr()-old(l.Repr()))
+  ensures allocated(l.Repr())
+  ensures {v} !! {l} + l.Repr()
+
   ensures l.Iterators() >= old(l.Iterators())
 
-  ensures forall x {:trigger x in l.Repr(), x in old(l.Repr())} | x in l.Repr() - old(l.Repr()) :: fresh(x)
-  ensures fresh(l.Repr()-old(l.Repr()))
-  ensures forall x | x in l.Repr() :: allocated(x)
-  ensures {v} !! {l} + l.Repr()
 {
   var it := l.Begin();
+  var b := it.HasNext();
 
   var i := 0;
-  while it.HasNext()
+  while b
     decreases |l.Model()| - it.Index()
     invariant l.Valid()
     invariant l.Model() == old(l.Model())
@@ -36,44 +39,47 @@ method FillArray<A>(l: List<A>, v: array<A>)
     invariant it.Index() == i
     invariant i <= |l.Model()|
     invariant v[..i] == l.Model()[..i]
+    invariant b == it.HasNext?()
+
+    invariant fresh(l.Repr()-old(l.Repr()))
+    invariant allocated(l.Repr())
 
     invariant l.Iterators() >= old(l.Iterators())
-
-    invariant forall x {:trigger x in l.Repr(), x in old(l.Repr())} | x in l.Repr() - old(l.Repr()) :: fresh(x)
-    invariant fresh(l.Repr()-old(l.Repr()))
-    invariant forall x | x in l.Repr() :: allocated(x)
   {
     var x := it.Next();
     v[i] := x;
+    b := it.HasNext();
     i := i + 1;
   }
 }
 
 method FillArrayLL<A>(l: LinkedList<A>, v: array<A>)
   modifies l, l.Repr(), v
+  requires allocated(l.Repr())
+
   requires {v} !! {l}
   requires {v} !! l.Repr()
   requires l.Valid()
   requires v.Length == |l.Model()|
-  requires forall x | x in l.Repr() :: allocated(x)
 
   ensures l.Valid()
   ensures l.Model() == old(l.Model())
   ensures v[..] == l.Model()
 
-  ensures l.Iterators() >= old(l.Iterators())
-  ensures forall it | it in old(l.Iterators()) && old(it.Valid()) :: it.Valid() && it.Index()==old(it.Index())
-
-  ensures forall x {:trigger x in l.Repr(), x in old(l.Repr())} | x in l.Repr() - old(l.Repr()) :: fresh(x)
   ensures fresh(l.Repr()-old(l.Repr()))
-  ensures forall x | x in l.Repr() :: allocated(x)
+  ensures allocated(l.Repr())
   ensures {v} !! {l} + l.Repr()
+
+
+  ensures l.Iterators() >= old(l.Iterators())
+  ensures forall it | it in old(l.Iterators()) && old(it.Valid()) :: it.Valid() && it.Parent()==old(it.Parent()) && it.Index()==old(it.Index())
 {
   ghost var iters:=l.Iterators();
   var it := l.Begin();
+  var b := it.HasNext();
 
   var i := 0;
-  while it.HasNext()
+  while b
     decreases |l.Model()| - it.Index()
     invariant l.Valid()
     invariant l.Model() == old(l.Model())
@@ -86,9 +92,14 @@ method FillArrayLL<A>(l: LinkedList<A>, v: array<A>)
     invariant it.Index() == i
     invariant i <= |l.Model()|
     invariant v[..i] == l.Model()[..i]
+    invariant b == it.HasNext?()
+
+    invariant fresh(l.Repr()-old(l.Repr()))
+    invariant allocated(l.Repr())
+
 
     invariant l.Iterators() >= old(l.Iterators())
-    invariant forall it | it in old(l.Iterators()) && old(it.Valid()) :: it.Valid() && it.Index()==old(it.Index())
+    invariant forall it | it in old(l.Iterators()) && old(it.Valid()) :: it.Valid() && it.Parent()==old(it.Parent()) && it.Index()==old(it.Index())
 
     invariant forall x {:trigger x in l.Repr(), x in old(l.Repr())} | x in l.Repr() - old(l.Repr()) :: fresh(x)
     invariant fresh(l.Repr()-old(l.Repr()))
@@ -97,35 +108,38 @@ method FillArrayLL<A>(l: LinkedList<A>, v: array<A>)
 
     var x := it.Next();
     v[i] := x;
+    b := it.HasNext();
     i := i + 1;
   }
 }
 
 method FillArrayAL<A>(l: ArrayList<A>, v: array<A>)
   modifies l, l.Repr(), v
+  requires allocated(l.Repr())
+
+  requires l.Valid()
   requires {v} !! {l}
   requires {v} !! l.Repr()
-  requires l.Valid()
   requires v.Length == |l.Model()|
-  requires forall x | x in l.Repr() :: allocated(x)
 
   ensures l.Valid()
   ensures l.Model() == old(l.Model())
   ensures v[..] == l.Model()
 
-  ensures l.Iterators() >= old(l.Iterators())
-  ensures forall it | it in old(l.Iterators()) && old(it.Valid()) :: it.Valid() && it.Index()==old(it.Index())
-
-  ensures forall x {:trigger x in l.Repr(), x in old(l.Repr())} | x in l.Repr() - old(l.Repr()) :: fresh(x)
   ensures fresh(l.Repr()-old(l.Repr()))
-  ensures forall x | x in l.Repr() :: allocated(x)
+  ensures allocated(l.Repr())
   ensures {v} !! {l} + l.Repr()
+
+  ensures l.Iterators() >= old(l.Iterators())
+  ensures forall it | it in old(l.Iterators()) && old(it.Valid()) :: it.Valid() && it.Parent()==old(it.Parent()) && it.Index()==old(it.Index())
+
 {
   ghost var iters := l.Iterators();
   var it := l.Begin();
+  var b := it.HasNext();
 
   var i := 0;
-  while it.HasNext()
+  while b
     decreases |l.Model()| - it.Index()
     invariant l.Valid()
     invariant l.Model() == old(l.Model())
@@ -138,16 +152,17 @@ method FillArrayAL<A>(l: ArrayList<A>, v: array<A>)
     invariant it.Index() == i
     invariant i <= |l.Model()|
     invariant v[..i] == l.Model()[..i]
+    invariant b == it.HasNext?()
+
+    invariant fresh(l.Repr()-old(l.Repr()))
+    invariant allocated(l.Repr())
 
     invariant l.Iterators() >= old(l.Iterators())
-    invariant forall it | it in old(l.Iterators()) && old(it.Valid()) :: it.Valid() && it.Index()==old(it.Index())
-
-    invariant forall x {:trigger x in l.Repr(), x in old(l.Repr())} | x in l.Repr() - old(l.Repr()) :: fresh(x)
-    invariant fresh(l.Repr()-old(l.Repr()))
-    invariant forall x | x in l.Repr() :: allocated(x)
+    invariant forall it | it in old(l.Iterators()) && old(it.Valid()) :: it.Valid() && it.Parent()==old(it.Parent()) && it.Index()==old(it.Index())
   {
     var x := it.Next();
     v[i] := x;
+    b := it.HasNext();
     i := i + 1;
   }
 }
