src/linear/layer1/List.dfy
@@ -25,7 +25,9 @@ trait ListIterator<A> {
     modifies this, Parent(), Parent().Repr()
     requires allocated(Parent())
     requires allocated(Parent().Repr())
-    
+    ensures fresh(Parent().Repr()-old(Parent().Repr()))
+    ensures allocated(Parent().Repr())
+
     requires Valid()
     requires Parent().Valid()
     ensures Valid()
@@ -35,9 +37,6 @@ trait ListIterator<A> {
     ensures Index()==old(Index())
     ensures b == HasNext?()
 
-    ensures fresh(Parent().Repr()-old(Parent().Repr()))
-    ensures allocated(Parent().Repr())
-
     ensures Parent().Iterators() >= old(Parent().Iterators())
     ensures forall it | it in old(Parent().Iterators()) && old(it.Valid()) ::
       it.Valid() && it.Parent() == old(it.Parent()) && it.Index() == old(it.Index())
@@ -46,7 +45,9 @@ trait ListIterator<A> {
     modifies this, Parent(), Parent().Repr()
     requires allocated(Parent())
     requires allocated(Parent().Repr())
-    
+    ensures fresh(Parent().Repr()-old(Parent().Repr()))
+    ensures allocated(Parent().Repr())
+
     requires Valid()
     requires Parent().Valid()
     requires HasNext?()
@@ -55,21 +56,19 @@ trait ListIterator<A> {
     ensures Parent() == old(Parent())  
     ensures Parent().Model() == old(Parent().Model())  
 
-    ensures fresh(Parent().Repr()-old(Parent().Repr()))
-    ensures allocated(Parent().Repr())
-
     ensures Parent().Iterators() >= old(Parent().Iterators())
     ensures x == Parent().Model()[old(Index())]
     ensures Index() == 1 + old(Index())
     ensures forall it | it in old(Parent().Iterators()) && old(it.Valid()) ::
       it.Valid() && it.Parent()==old(it.Parent()) && (it != this ==> it.Index() == old(it.Index()))
-
   
   method Peek() returns (p:A)
     modifies this, Parent(), Parent().Repr()
     requires allocated(Parent())
     requires allocated(Parent().Repr())
-    
+    ensures fresh(Parent().Repr()-old(Parent().Repr()))
+    ensures allocated(Parent().Repr())
+
     requires Valid()
     requires Parent().Valid()
     requires HasNext?()
@@ -80,19 +79,17 @@ trait ListIterator<A> {
     ensures Index() == old(Index())
     ensures p==Parent().Model()[Index()] 
     
-    ensures fresh(Parent().Repr()-old(Parent().Repr()))
-    ensures allocated(Parent().Repr())
-
     ensures Parent().Iterators() >= old(Parent().Iterators())
     ensures forall it | it in old(Parent().Iterators()) && old(it.Valid()) ::
       it.Valid() && it.Parent()==old(it.Parent()) && it.Index() == old(it.Index())
-
 
   method Copy() returns (it: ListIterator<A>)
     modifies this, Parent(), Parent().Repr()
     requires allocated(Parent())
     requires allocated(Parent().Repr())
-    
+    ensures fresh(Parent().Repr()-old(Parent().Repr()))
+    ensures allocated(Parent().Repr())
+
     requires Valid()
     requires Parent().Valid()
     ensures fresh(it)
@@ -101,9 +98,6 @@ trait ListIterator<A> {
     ensures Parent() == old(Parent())
     ensures Parent().Model() == old(Parent().Model())
     ensures Index()==old(Index())
-
-    ensures fresh(Parent().Repr()-old(Parent().Repr()))
-    ensures allocated(Parent().Repr())
     
     ensures it.Valid()
     ensures Parent().Iterators() >= {it} + old(Parent().Iterators())
@@ -116,7 +110,9 @@ trait ListIterator<A> {
     modifies this, Parent(), Parent().Repr()
     requires allocated(Parent())
     requires allocated(Parent().Repr())
-   
+    ensures fresh(Parent().Repr()-old(Parent().Repr()))
+    ensures allocated(Parent().Repr())
+
     requires Valid()
     requires Parent().Valid()
     requires HasNext?()
@@ -126,9 +122,6 @@ trait ListIterator<A> {
     ensures |Parent().Model()| == old(|Parent().Model()|)
     ensures Index() == old(Index()) 
     ensures Parent().Model()==old(Parent().Model()[Index():=x])
-    
-    ensures fresh(Parent().Repr()-old(Parent().Repr()))
-    ensures allocated(Parent().Repr())
 
     ensures Parent().Iterators() >= old(Parent().Iterators())
     ensures forall it | it in old(Parent().Iterators()) && old(it.Valid()) ::
@@ -144,28 +137,26 @@ trait List<A> extends ADT<seq<A>> {
   method Empty() returns (b:bool)
     modifies this, Repr()
     requires allocated(Repr())
+    ensures fresh(Repr()-old(Repr()))
+    ensures allocated(Repr())
     
     requires Valid()
     ensures Valid()
     ensures Model() == old(Model())
     ensures b==Empty?() 
 
-    ensures fresh(Repr()-old(Repr()))
-    ensures allocated(Repr())
- 
     ensures Iterators() >= old(Iterators())
 
   method Size() returns (s:nat)
     modifies this, Repr()
     requires allocated(Repr())
+    ensures fresh(Repr()-old(Repr()))
+    ensures allocated(Repr())
     
     requires Valid()
     ensures Valid()
     ensures Model() == old(Model())
     ensures s==|Model()| 
-
-    ensures fresh(Repr()-old(Repr()))
-    ensures allocated(Repr())
 
     ensures Iterators() >= old(Iterators())
 
@@ -177,13 +168,12 @@ trait List<A> extends ADT<seq<A>> {
   method Begin() returns (it: ListIterator<A>)
     modifies this, Repr()
     requires allocated(Repr())
-    
+    ensures fresh(Repr()-old(Repr()))
+    ensures allocated(Repr())
+ 
     requires Valid()
     ensures Valid()
     ensures Model() == old(Model())
-
-    ensures fresh(Repr()-old(Repr()))
-    ensures allocated(Repr())
 
     ensures fresh(it)
     ensures Iterators() >= {it} + old(Iterators())
@@ -196,84 +186,78 @@ trait List<A> extends ADT<seq<A>> {
   method Front() returns (x:A)
     modifies this, Repr()
     requires allocated(Repr())
-    
+    ensures fresh(Repr()-old(Repr()))
+    ensures allocated(Repr())
+ 
     requires Valid()
     requires !Empty?()
     ensures Valid()
     ensures Model() == old(Model())
     ensures x == Model()[0]
-
-    ensures fresh(Repr()-old(Repr()))
-    ensures allocated(Repr())
  
     ensures Iterators() >= old(Iterators())
   
   method PushFront(x: A)
     modifies this, Repr()
     requires allocated(Repr())
-    
+    ensures fresh(Repr()-old(Repr()))
+    ensures allocated(Repr())
+
     requires Valid()
     ensures Valid()
     ensures Model() == [x] + old(Model())
-
-    ensures fresh(Repr()-old(Repr()))
-    ensures allocated(Repr())
 
     ensures Iterators() >= old(Iterators())
 
   method PopFront() returns (x: A)
     modifies this, Repr()
     requires allocated(Repr())
-   
+    ensures fresh(Repr()-old(Repr()))
+    ensures allocated(Repr())
+
     requires Valid()
     requires !Empty?()
     ensures Valid()
     ensures [x] + Model() == old(Model())
 
+    ensures Iterators() >= old(Iterators())
+
+  method Back() returns (x:A)
+    modifies this, Repr()
+    requires allocated(Repr())
     ensures fresh(Repr()-old(Repr()))
     ensures allocated(Repr())
 
-    ensures Iterators() >= old(Iterators())
-
-  method Back() returns (x:A)//Nuevo metodo
-    modifies this, Repr()
-    requires allocated(Repr())
-    
     requires Valid()
     requires !Empty?()
     ensures Valid()
     ensures Model() == old(Model())
     ensures x == Model()[|Model()|-1]
 
-    ensures fresh(Repr()-old(Repr()))
-    ensures allocated(Repr())
- 
     ensures Iterators() >= old(Iterators())
   
   method PushBack(x: A)
     modifies this, Repr()
     requires allocated(Repr())
-    
+    ensures fresh(Repr()-old(Repr()))
+    ensures allocated(Repr())
+
     requires Valid()
     ensures Valid()
     ensures Model() == old(Model()) + [x]
-
-    ensures fresh(Repr()-old(Repr()))
-    ensures allocated(Repr())
 
     ensures Iterators() >= old(Iterators())
 
   method PopBack() returns (x: A)
     modifies this, Repr()
     requires allocated(Repr())
-    
+    ensures fresh(Repr()-old(Repr()))
+    ensures allocated(Repr())
+
     requires Valid()
     requires !Empty?()
     ensures Valid()
     ensures Model() + [x] == old(Model())
-
-    ensures fresh(Repr()-old(Repr()))
-    ensures allocated(Repr())
 
     ensures Iterators() >= old(Iterators())
 
@@ -281,6 +265,8 @@ trait List<A> extends ADT<seq<A>> {
   method Insert(mid: ListIterator<A>, x: A) returns (newt: ListIterator<A>)
     modifies this, Repr()
     requires allocated(Repr())
+    ensures fresh(Repr()-old(Repr()))
+    ensures allocated(Repr())
 
     requires Valid()
     requires mid.Valid()
@@ -288,9 +274,6 @@ trait List<A> extends ADT<seq<A>> {
     requires mid in Iterators()
     ensures Valid()
     ensures Model() == Seq.Insert(x, old(Model()), old(mid.Index()))
-
-    ensures fresh(Repr()-old(Repr()))
-    ensures allocated(Repr())
 
     ensures fresh(newt)
     ensures Iterators() >= {newt}+old(Iterators())
@@ -301,6 +284,8 @@ trait List<A> extends ADT<seq<A>> {
   method Erase(mid: ListIterator<A>) returns (next: ListIterator<A>)
     modifies this, Repr()
     requires allocated(Repr())
+    ensures fresh(Repr()-old(Repr()))
+    ensures allocated(Repr())
 
     requires Valid()
     requires mid.Valid()
@@ -309,9 +294,6 @@ trait List<A> extends ADT<seq<A>> {
     requires mid in Iterators()
     ensures Valid()
     ensures Model() == Seq.Remove(old(Model()), old(mid.Index()))
-
-    ensures fresh(Repr()-old(Repr()))
-    ensures allocated(Repr())
 
     ensures fresh(next)
     ensures Iterators() >= {next}+old(Iterators())
